WIP type constructors
cannot handle quantifiers by substuting value expressions, since abstract values cannot be captured by expressions

BoogieLang/Binders.thy
@@ -6,17 +6,18 @@ fun vopen :: "nat \<Rightarrow> vname \<Rightarrow> expr \<Rightarrow> expr"
   where 
     "vopen k x (BVar i) = (if (i = k) then (Var x) else (BVar i))"
   | "vopen k x (Var y) = Var x"
-  | "vopen k x (Val v) = Val v"
+  | "vopen k x (Lit l) = Lit l"
   | "vopen k x (UnOp uop e) = (UnOp uop (vopen k x e))"
   | "vopen k x (e1 \<guillemotleft>bop\<guillemotright> e2) = (vopen k x e1) \<guillemotleft>bop\<guillemotright> (vopen k x e2)"
   | "vopen k x (FunExp f es) = (FunExp f (map (vopen k x) es))"
   | "vopen k x (Forall ty e) = (Forall ty (vopen (k+1) x e))"
+  | "vopen k x (Exists ty e) = (Exists ty (vopen (k+1) x e))"
 
 fun eopen :: "nat \<Rightarrow> expr \<Rightarrow> expr \<Rightarrow> expr"
   where 
     "eopen k e' (BVar i) = (if (i = k) then e' else (BVar i))"
   | "eopen k e' (Var y) = Var y"
-  | "eopen k e' (Val v) = Val v"
+  | "eopen k e' (Lit l) = Lit l"
   | "eopen k e' (UnOp uop e) = (UnOp uop (eopen k e' e))"
   | "eopen k e' (e1 \<guillemotleft>bop\<guillemotright> e2) = (eopen k e' e1) \<guillemotleft>bop\<guillemotright> (eopen k e' e2)"
   | "eopen k e' (FunExp f es) = (FunExp f (map (eopen k e') es))"
@@ -27,7 +28,7 @@ inductive lc :: "expr \<Rightarrow> bool" and
    lc_list :: "expr list \<Rightarrow> bool"
   where 
    "lc (Var y)"
- | "lc (Val v)"
+ | "lc (Lit l)"
  | "lc e \<Longrightarrow> lc (UnOp uop e)"
  | "\<lbrakk>lc e1; lc e2\<rbrakk> \<Longrightarrow> lc (e1 \<guillemotleft>bop\<guillemotright> e2)"
  | "lc_list es \<Longrightarrow> lc (FunExp f es)"
@@ -39,20 +40,22 @@ fun lc_at :: "nat \<Rightarrow> expr \<Rightarrow> bool"
   where
    "lc_at k (Var y) = True"
  | "lc_at k (BVar i) = (i < k)"
- | "lc_at k (Val v) = True"
+ | "lc_at k (Lit l) = True"
  | "lc_at k (UnOp uop e) = lc_at k e"
  | "lc_at k (e1 \<guillemotleft>bop\<guillemotright> e2) = (lc_at k e1 \<and> lc_at k e2)"
  | "lc_at k (FunExp f es) = list_all (lc_at k) es"
  | "lc_at k (Forall ty e) = lc_at (k+1) e"
+ | "lc_at k (Exists ty e) = lc_at (k+1) e"
 
 fun fv :: "expr \<Rightarrow> vname set"
   where
     "fv (BVar i) = {}"
   | "fv (Var y) = {y}"
-  | "fv (Val v) = {}"
+  | "fv (Lit l) = {}"
   | "fv (UnOp up e) = fv e"
   | "fv (e1 \<guillemotleft>bop\<guillemotright> e2) = (fv e1) \<union> (fv e2)"
   | "fv (FunExp f es) = fold (union \<circ> fv) es {}"
   | "fv (Forall ty e) = fv e"
-
+  | "fv (Exists ty e) = fv e"
+  
 end
